finally get the proof of set done

cedar-dafny/pe/util.dfy
@@ -17,6 +17,35 @@ module pe.util {
     => f(xs[i]))
   }
 
+  lemma MapExists<T,R>(xs: seq<T>, f: (T --> R), p: (R -> bool))
+    requires forall i :: 0 <= i < |xs| ==> f.requires(xs[i])
+    requires exists x | x in xs :: p(f(x))
+    ensures exists y | y in Map(xs, f) :: p(y) {
+    assert Map(xs, f) == seq(|xs|, i requires 0 <= i < |xs| && f.requires(xs[i]) => f(xs[i]));
+    assert exists i: nat | i < |xs| :: p(f(xs[i]));
+    assert exists i: nat | i < |xs| :: Map(xs, f)[i] == f(xs[i]);
+    var i: nat :| i < |xs| && Map(xs, f)[i] == f(xs[i]);
+  }
+
+  lemma MapEqvFunc<A,B>(xs: seq<A>, f: (A --> B), g: (A --> B))
+    requires forall i :: 0 <= i < |xs| ==> f.requires(xs[i]) && g.requires(xs[i]) && f(xs[i]) == g(xs[i])
+    ensures Map(xs, f) == Map(xs, g)
+  {
+
+  }
+
+  lemma MapCompose<T, X, Y>(es: seq<T>, f: (T --> X), g: (X -> Y))
+    requires forall i :: 0 <= i < |es| ==> f.requires(es[i])
+    ensures Map(Map(es, f), g) == Map(es, e requires f.requires(e) => g(f(e))) {
+    if |es| == 0 {
+      assume false;
+    } else {
+      MapCompose(es[1..], f, g);
+      assert Map(Map(es, f), g) == Map([f(es[0])] + Map(es[1..], f), g) == [g(f(es[0]))] + Map(Map(es[1..], f), g);
+      assert Map(es, e requires f.requires(e) => g(f(e))) == [g(f(es[0]))] + Map(es[1..], e requires f.requires(e) => g(f(e)));
+    }
+  }
+
   function CollectToSet<T,E>(rs: seq<Result<T, E>>): (result: Result<set<T>,E>) {
     if |rs| == 0 then
       Ok({})
@@ -24,5 +53,54 @@ module pe.util {
       var x :- rs[0];
       var xs :- CollectToSet(rs[1..]);
       Ok({x} + xs)
+  }
+
+  lemma CollectToSetErr<T,E>(rs: seq<Result<T, E>>)
+    requires exists r | r in rs :: r.Err?
+    ensures CollectToSet(rs).Err? {
+
+  }
+
+  lemma CollectToSetOk<T,E>(rs: seq<std.Result<T, E>>)
+    requires forall r | r in rs :: r.Ok?
+    ensures var res := CollectToSet(rs); res.Ok? && res.value == set x | x in rs :: x.value
+  {
+
+  }
+
+  lemma CollectToSetWithMap<T,E, U>(rs: seq<T>, f: T--> Result<U, E>)
+    requires forall r | r in rs :: f.requires(r) && f(r).Ok?
+    ensures var res := CollectToSet(Map(rs, f)); res.Ok? && res.value == set x | x in rs :: f(x).value
+  {
+    if |rs| == 0 {
+
+    } else {
+      CollectToSetWithMap(rs[1..], f);
+      assert Map(rs, f) == [f(rs[0])] + Map(rs[1..], f);
+    }
+
+  }
+
+  function CollectToSeq<T,E>(rs: seq<Result<T, E>>): (result: Result<seq<T>,E>) {
+    if |rs| == 0 then
+      Ok([])
+    else
+      var x :- rs[0];
+      var xs :- CollectToSeq(rs[1..]);
+      Ok([x] + xs)
+  }
+
+  lemma CollectToSeqOk<T,E>(rs: seq<std.Result<T, E>>)
+    requires forall r | r in rs :: r.Ok?
+    ensures var res := CollectToSeq(rs); res.Ok? && res.value == Map(rs, (r: std.Result<T, E>) requires r.Ok? => r.value) {
+    if |rs| == 0 {
+      assert CollectToSeq(rs) == Ok([]);
+      assert Map(rs, (r: std.Result<T, E>) requires r.Ok? => r.value) == [];
+    } else {
+      CollectToSeqOk(rs[1..]);
+      assert CollectToSeq(rs).value == [rs[0].value] + CollectToSeq(rs[1..]).value;
+      assert Map(rs, (r: std.Result<T, E>) requires r.Ok? => r.value) ==
+             [rs[0].value] + Map(rs[1..], (r: std.Result<T, E>) requires r.Ok? => r.value);
+    }
   }
 }
