cedar-dafny/pe/eval.dfy
@@ -1,6 +1,7 @@
 include "def.dfy"
 include "util.dfy"
 include "environment.dfy"
+include "engine.dfy"
 include "../def/core.dfy"
 include "../def/base.dfy"
 include "../def/engine.dfy"
@@ -13,7 +14,92 @@ module pe.eval {
   import def.base
   import opened def.std
   import util
-  import environment
+  import opened environment
+  import opened engine
+
+  lemma MakeErrorValueIsErr(env: Environment)
+    requires env.wellFormed()
+    ensures var r := PartialEvaluator.makeErrorValue(); env.interpret(r, core.EntityStore(map[])).Err? {
+    calc {
+      env.interpret(PartialEvaluator.makeErrorValue(), core.EntityStore(map[]));
+    ==
+      calc {
+        env.interpret(Residual.Record([]), core.EntityStore(map[]));
+      ==
+        Ok(core.Value.Record(map[]));
+      }
+      Err(base.AttrDoesNotExist);
+    }
+  }
+
+  lemma InterpretRestrictedResidualSet(rs: seq<Residual>, env: Environment, s: core.EntityStore)
+    requires forall r | r in rs :: r.restricted?()
+    requires env.wellFormed()
+    ensures env.interpretSet(rs, s) == env.interpretSet(rs, core.EntityStore(map[]))
+  {
+    if |rs| == 0 {
+
+    } else {
+      InterpretRestrictedResidual(rs[0], env, s);
+    }
+  }
+
+  lemma InterpretRestrictedResidualRecord(bs: seq<(core.Attr, Residual)>, env: Environment, s: core.EntityStore)
+    requires forall b | b in bs :: b.1.restricted?()
+    requires env.wellFormed()
+    ensures env.interpretRecord(bs, s) == env.interpretRecord(bs, core.EntityStore(map[]))
+  {
+    if |bs| == 0 {
+
+    } else {
+      InterpretRestrictedResidual(bs[0].1, env, s);
+    }
+  }
+
+  lemma InterpretRestrictedResidualList(rs: seq<Residual>, env: Environment, s: core.EntityStore)
+    requires forall r | r in rs :: r.restricted?()
+    requires env.wellFormed()
+    ensures env.interpretList(rs, s) == env.interpretList(rs, core.EntityStore(map[])) {
+    if |rs| == 0 {
+
+    } else {
+      InterpretRestrictedResidual(rs[0], env, s);
+    }
+  }
+
+  lemma InterpretRestrictedResidual(r: Residual, env: Environment, s: core.EntityStore)
+    requires r.restricted?()
+    requires env.wellFormed()
+    ensures env.interpret(r, s) == env.interpret(r, core.EntityStore(map[]))
+  {
+    match r {
+      case Concrete(_) =>
+      case Unknown(_) =>
+      case Set(rs) => InterpretRestrictedResidualSet(rs, env, s);
+      case Record(bs) => InterpretRestrictedResidualRecord(bs, env, s);
+      case Call(_, args) => InterpretRestrictedResidualList(args, env, s);
+      case _ => assume false;
+    }
+  }
+
+  lemma PEInterpretSeqErr(es: seq<definition.Expr>, pe: PartialEvaluator)
+    requires pe.interpretSeq(es).Err?
+    ensures exists e | e in es :: pe.interpret(e).Err?
+  {
+
+  }
+
+  lemma CEInterpretSetErr(es: seq<core.Expr>, ce: ce.Evaluator)
+    requires exists e | e in es :: ce.interpret(e).Err?
+    ensures ce.interpretSet(es).Err? {
+
+  }
+
+  lemma CEInterpretSetOk(es: seq<core.Expr>, ce: ce.Evaluator)
+    requires ce.interpretSet(es).Ok?
+    ensures forall e | e in es :: ce.interpret(e).Ok? {
+
+  }
 
   lemma CEInterpretSetMapReduce(es: seq<core.Expr>, ce: ce.Evaluator)
     ensures ce.interpretSet(es) == util.CollectToSet(util.Map(es, ce.interpret))
@@ -23,24 +109,77 @@ module pe.eval {
     }
   }
 
-  lemma MapCompose<T, X, Y>(es: seq<T>, f: (T --> X), g: (X -> Y))
-    requires forall i :: 0 <= i < |es| ==> f.requires(es[i])
-    ensures util.Map(util.Map(es, f), g) == util.Map(es, e requires f.requires(e) => g(f(e))) {
-    if |es| == 0 {
-      assume false;
+  lemma EnvInterpretSetMapReduce(rs: seq<Residual>, env: environment.Environment, s: core.EntityStore)
+    requires env.wellFormed()
+    ensures env.interpretSet(rs, s) == util.CollectToSet(util.Map(rs, r => env.interpret(r, s)))
+  {
+    if |rs| == 0 {
+
     } else {
-      MapCompose(es[1..], f, g);
-      assert util.Map(util.Map(es, f), g) == util.Map([f(es[0])] + util.Map(es[1..], f), g) == [g(f(es[0]))] + util.Map(util.Map(es[1..], f), g);
-      assert util.Map(es, e requires f.requires(e) => g(f(e))) == [g(f(es[0]))] + util.Map(es[1..], e requires f.requires(e) => g(f(e)));
+      assert util.Map(rs, r => env.interpret(r, s)) == [env.interpret(rs[0], s)] + util.Map(rs[1..], r => env.interpret(r, s));
+    }
+  }
+
+  lemma PEInterpretSeqOk(es: seq<definition.Expr>, pe: PartialEvaluator)
+    requires pe.interpretSeq(es).Ok?
+    ensures forall e | e in es :: pe.interpret(e).Ok?
+  {
+
+  }
+
+  lemma PEInterpretSetMapReduce(es: seq<definition.Expr>, pe: PartialEvaluator)
+    ensures pe.interpretSeq(es) == util.CollectToSeq(util.Map(es, pe.interpret))
+  {
+    if |es| > 0 {
+      assert util.Map(es, pe.interpret) == [pe.interpret(es[0])] + util.Map(es[1..], pe.interpret);
+    }
+  }
+
+  lemma PEInterpretSet(e: definition.Expr, PE: PartialEvaluator, env: environment.Environment, s: core.EntityStore)
+    requires e.Set?
+    requires env.wellFormed()
+    requires PE.interpretSeq(e.es).Ok?
+    requires !forall r | r in PE.interpretSeq(e.es).value :: r.Concrete?
+    ensures (forall i: nat | i < |e.es| :: PE.interpret(e.es[i]).Ok?) && env.interpret(PE.interpret(e).value, s) == util.CollectToSet(util.Map(e.es, e' requires PE.interpret(e').Ok? => env.interpret(PE.interpret(e').value, s))).Map(v => core.Value.Set(v)) {
+    PEInterpretSeqOk(e.es, PE);
+    assert forall e' | e' in e.es :: PE.interpret(e').Ok?;
+    assert forall i: nat | i < |e.es| :: PE.interpret(e.es[i]).Ok?;
+    PEInterpretSetMapReduce(e.es, PE);
+    util.CollectToSeqOk(util.Map(e.es, PE.interpret));
+    var peI := e requires PE.interpret(e).Ok? => PE.interpret(e).value;
+    calc == {
+      PE.interpretSeq(e.es).value;
+      util.CollectToSeq(util.Map(e.es, PE.interpret)).value;
+      util.Map(util.Map(e.es, PE.interpret), (r: definition.Result<Residual>) requires r.Ok? => r.value);
+      util.Map(e.es, peI);
+    }
+    EnvInterpretSetMapReduce(util.Map(e.es, peI), env, s);
+    calc == {
+      env.interpretSet(PE.interpretSeq(e.es).value, s);
+      env.interpretSet(util.Map(e.es, peI), s);
+      util.CollectToSet(util.Map(util.Map(e.es, peI), r => env.interpret(r, s)));
+    }
+    assert util.CollectToSet(util.Map(e.es, e requires PE.interpret(e).Ok? => env.interpret(PE.interpret(e).value, s))) == util.CollectToSet(util.Map(util.Map(e.es, peI), r => env.interpret(r, s))) by {
+      util.MapCompose(e.es, peI, r => env.interpret(r, s));
+      assert util.Map(util.Map(e.es, peI), r => env.interpret(r, s)) == util.Map(e.es, e requires PE.interpret(e).Ok? => env.interpret(PE.interpret(e).value, s));
+    }
+    calc == {
+      env.interpret(PE.interpret(e).value, s);
+      env.interpret(Residual.Set(PE.interpretSeq(e.es).value), s);
+      env.interpretSet(PE.interpretSeq(e.es).value, s).Map(v => core.Value.Set(v));
     }
   }
 
   lemma CEInterpretSet(e: definition.Expr, CE: ce.Evaluator, env: environment.Environment)
     requires e.Set?
     requires env.wellFormed()
-    ensures CE.interpret(env.replaceUnknownInExpr(e)) == util.CollectToSet(util.Map(e.es, e' requires e' < e => CE.interpret(env.replaceUnknownInExpr(e')))).Map(v => core.Value.Set(v)) {
+    ensures CE.interpret(env.replaceUnknownInExpr(e)) ==
+            util.CollectToSet(
+              util.Map(
+                e.es,
+                e' requires e' < e => CE.interpret(env.replaceUnknownInExpr(e')))).Map(v => core.Value.Set(v)) {
     CEInterpretSetMapReduce(util.Map(e.es, e' requires e' < e => env.replaceUnknownInExpr(e')), CE);
-    MapCompose(e.es, e' requires e' < e => env.replaceUnknownInExpr(e'), CE.interpret);
+    util.MapCompose(e.es, e' requires e' < e => env.replaceUnknownInExpr(e'), CE.interpret);
     assert util.Map(util.Map(e.es, e' requires e' < e => env.replaceUnknownInExpr(e')), CE.interpret) == util.Map(e.es, e' requires e' < e => CE.interpret(env.replaceUnknownInExpr(e')));
     calc == {
       CE.interpret(env.replaceUnknownInExpr(e));
